Finish commsq.bicartesian_iff_isos

src/for_mathlib/bicartesian3.lean
@@ -34,44 +34,177 @@ variables (sqₗ : commsq ιh₁ gKh g₁ ιh₂) (sqm : commsq f₁ g₁ g₂ f
 variables (sqᵣ : commsq πh₁ g₂ gQh πh₂)
 variables (sqₛ : commsq f₂ πv₁ πv₂ fQv)
 
-include H₁ H₂ sqₗ sqm sqᵣ
-
 open_locale zero_object
 open category_theory.abelian
+
+def is_limit_of_is_limit_comp {X Y Z : 𝓐} {f : X ⟶ Y} {g : Y ⟶ Z}
+  {c : kernel_fork (f ≫ g)} (hc : is_limit c) (h : c.ι ≫ f = 0) :
+  is_limit (kernel_fork.of_ι c.ι h) :=
+is_limit.of_ι _ _
+  (λ T l hl, hc.lift (kernel_fork.of_ι l (by rw [reassoc_of hl, zero_comp])))
+  (λ T l hl, hc.fac _ _)
+  (λ T l hl m hm, fork.is_limit.hom_ext hc (by { erw [hm, hc.fac], refl }))
+
+def is_colimit_of_is_colimit_comp {X Y Z : 𝓐} {f : X ⟶ Y} {g : Y ⟶ Z}
+  {c : cokernel_cofork (f ≫ g)} (hc : is_colimit c) (h : g ≫ c.π = 0) :
+  is_colimit (cokernel_cofork.of_π c.π h) :=
+is_colimit.of_π _ _
+  (λ T l hl, hc.desc (cokernel_cofork.of_π l (by rw [category.assoc, hl, comp_zero])))
+  (λ T l hl, hc.fac _ _)
+  (λ T l hl m hm, cofork.is_colimit.hom_ext hc (by { erw [hm, hc.fac], refl }))
+
+section
+include sqₗ sqm
+
+lemma is_iso_of_is_limit (H₁ : exact ιh₁ f₁) (H₂ : exact ιh₂ f₂)
+  (h : is_limit (pullback_cone.mk f₁ g₁ sqm.w)) : is_iso gKh :=
+begin
+  haveI : mono gKh,
+  { refine preadditive.mono_of_cancel_zero _ (λ P g hg, _),
+    apply zero_of_comp_mono ιh₁,
+    apply pullback_cone.is_limit.hom_ext h,
+    { rw [pullback_cone.mk_fst, category.assoc, zero_comp, H₁.w, comp_zero] },
+    { rw [pullback_cone.mk_snd, category.assoc, sqₗ.w, ← category.assoc, hg, zero_comp,
+        zero_comp] } },
+  obtain ⟨l, hl₁, hl₂ : l ≫ g₁ = _⟩ :=
+    pullback_cone.is_limit.lift' h 0 ιh₂ (by simp [H₂.w]),
+  let ker := is_limit_of_exact_of_mono _ _ H₁,
+  obtain ⟨inv, hinv : inv ≫ ιh₁ = l⟩ := kernel_fork.is_limit.lift' ker l hl₁,
+  have hinv' : inv ≫ gKh = 𝟙 _,
+   { rw [← cancel_mono ιh₂, category.assoc, ← sqₗ.w, reassoc_of hinv, hl₂, category.id_comp] },
+  refine ⟨⟨inv, _, hinv'⟩⟩,
+  rw [← cancel_mono gKh, category.assoc, hinv', category.comp_id, category.id_comp]
+end
+
+end
+
+section
+include sqm sqᵣ
+
+lemma is_iso_of_is_colimit (H₁ : exact f₁ πh₁) (H₂ : exact f₂ πh₂)
+  (h : is_colimit (pushout_cocone.mk _ _ sqm.w)) : is_iso gQh :=
+begin
+  haveI : epi gQh,
+  { refine preadditive.epi_of_cancel_zero _ (λ P g hg, _),
+    apply zero_of_epi_comp πh₂,
+    apply pushout_cocone.is_colimit.hom_ext h,
+    { rw [pushout_cocone.mk_inl, ← category.assoc, ← sqᵣ.w, category.assoc, hg, comp_zero,
+        comp_zero] },
+    { rw [pushout_cocone.mk_inr, ← category.assoc, H₂.w, comp_zero, zero_comp] } },
+  obtain ⟨l, hl₁ : g₂ ≫ l = _, hl₂⟩ :=
+    pushout_cocone.is_colimit.desc' h πh₁ 0 (by simp [H₁.w]),
+  let coker := is_colimit_of_exact_of_epi _ _ H₂,
+  obtain ⟨inv, hinv : πh₂ ≫ inv = l⟩ := cokernel_cofork.is_colimit.desc' coker l hl₂,
+  have hinv' : gQh ≫ inv = 𝟙 _,
+  { rw [← cancel_epi πh₁, ← category.assoc, sqᵣ.w, category.assoc, hinv, hl₁, category.comp_id] },
+  refine ⟨⟨inv, hinv', _⟩⟩,
+  rw [← cancel_epi gQh, reassoc_of hinv', category.comp_id]
+end
+
+end
+
+include H₁ H₂ sqₗ sqm sqᵣ
 
 lemma commsq.bicartesian_iff_isos : sqm.bicartesian ↔ (is_iso gKh ∧ is_iso gQh) :=
 begin
   split,
   { intro h, split,
-    { haveI : mono gKh,
-      { refine preadditive.mono_of_cancel_zero _ (λ P g hg, _),
-        apply zero_of_comp_mono ιh₁,
-        apply pullback_cone.is_limit.hom_ext h.is_limit,
-        { rw [pullback_cone.mk_fst, category.assoc, zero_comp, (H₁.extract 0 2).w, comp_zero] },
-        { rw [pullback_cone.mk_snd, category.assoc, sqₗ.w, ← category.assoc, hg, zero_comp,
-            zero_comp] } },
-        obtain ⟨l, hl₁, hl₂ : l ≫ g₁ = _⟩ :=
-          pullback_cone.is_limit.lift' h.is_limit 0 ιh₂ (by simp [(H₂.extract 0 2).w]),
-        let ker := is_limit_of_exact_of_mono _ _ ((exact_iff_exact_seq _ _).2 (H₁.extract 0 2)),
-        obtain ⟨inv, hinv : inv ≫ ιh₁ = l⟩ := kernel_fork.is_limit.lift' ker l hl₁,
-        have hinv' : inv ≫ gKh = 𝟙 _,
-        { rw [← cancel_mono ιh₂, category.assoc, ← sqₗ.w, reassoc_of hinv, hl₂, category.id_comp] },
-        refine ⟨⟨inv, _, hinv'⟩⟩,
-        rw [← cancel_mono gKh, category.assoc, hinv', category.comp_id, category.id_comp] },
-    { haveI : epi gQh,
-      { refine preadditive.epi_of_cancel_zero _ (λ P g hg, _),
-        apply zero_of_epi_comp πh₂,
-        apply pushout_cocone.is_colimit.hom_ext h.is_colimit,
-        { rw [pushout_cocone.mk_inl, ← category.assoc, ← sqᵣ.w, category.assoc, hg, comp_zero,
-            comp_zero] },
-        { rw [pushout_cocone.mk_inr, ← category.assoc, (H₂.extract 1 2).w, comp_zero, zero_comp] } },
-      obtain ⟨l, hl₁ : g₂ ≫ l = _, hl₂⟩ :=
-        pushout_cocone.is_colimit.desc' h.is_colimit πh₁ 0 (by simp [(H₁.extract 1 2).w]),
-      let coker := is_colimit_of_exact_of_epi _ _ ((exact_iff_exact_seq _ _).2 (H₂.extract 1 2)),
-      obtain ⟨inv, hinv : πh₂ ≫ inv = l⟩ := cokernel_cofork.is_colimit.desc' coker l hl₂,
-      have hinv' : gQh ≫ inv = 𝟙 _,
-      { rw [← cancel_epi πh₁, ← category.assoc, sqᵣ.w, category.assoc, hinv, hl₁, category.comp_id] },
-      refine ⟨⟨inv, hinv', _⟩⟩,
-      rw [← cancel_epi gQh, reassoc_of hinv', category.comp_id] } },
-  { sorry }
+    { exact is_iso_of_is_limit gKh sqₗ sqm ((exact_iff_exact_seq _ _).2 (H₁.extract 0 2))
+      ((exact_iff_exact_seq _ _).2 (H₂.extract 0 2)) h.is_limit },
+    { exact is_iso_of_is_colimit gQh sqm sqᵣ ((exact_iff_exact_seq _ _).2 (H₁.extract 1 2))
+      ((exact_iff_exact_seq _ _).2 (H₂.extract 1 2)) h.is_colimit } },
+  { rintros ⟨gKh_iso, gQh_iso⟩,
+    resetI,
+    apply commsq.bicartesian.of_is_limit_of_is_colimt,
+    { apply is_limit.of_point_iso (limit.is_limit _),
+      { apply_instance },
+      { let r := pullback.lift _ _ sqm.w,
+        let x : Kh₁ ⟶ kernel (pullback.fst : pullback g₂ f₂ ⟶ A₁₂),
+        { refine kernel.lift _ (ιh₁ ≫ r) _,
+          simp only [(H₁.extract 0 2).w, category.assoc, pullback.lift_fst] },
+        haveI : is_iso x,
+        { let psq := commsq.of_eq (@pullback.condition _ _ _ _ _ g₂ f₂ _),
+          let hker := abelian.is_limit_of_exact_of_mono _ _
+            ((exact_iff_exact_seq _ _).2 (H₂.extract 0 2)),
+          obtain ⟨u : _ ⟶ Kh₂, hu⟩ := kernel_fork.is_limit.lift' hker
+            (kernel.ι (pullback.fst : pullback g₂ f₂ ⟶ A₁₂) ≫ pullback.snd) _,
+          { rw fork.ι_of_ι at hu,
+            let lsq := commsq.of_eq hu.symm,
+            haveI : is_iso u := is_iso_of_is_limit u lsq psq _ _ _,
+            { have hxu : x ≫ u = gKh,
+              { simp only [← cancel_mono ιh₂, category.assoc, hu, x, kernel.lift_ι_assoc, r,
+                pullback.lift_snd, sqₗ.w] },
+              have hx : x = gKh ≫ inv u,
+              { rw [← is_iso.comp_inv_eq, is_iso.inv_inv, hxu] },
+              rw hx,
+              apply_instance },
+            { exact exact_kernel_ι },
+            { exact ((exact_iff_exact_seq _ _).2 (H₂.extract 0 2)) },
+            { exact pullback_is_pullback _ _ } },
+          { rw [category.assoc, ← pullback.condition, kernel.condition_assoc, zero_comp] } },
+        refine @abelian.is_iso_of_is_iso_of_is_iso_of_is_iso_of_is_iso _ _ _ 0 _ _ _ 0 _ _ _
+         0 ιh₁ f₁ 0 (kernel.ι (pullback.fst : pullback g₂ f₂ ⟶ A₁₂)) pullback.fst 0 x r (𝟙 _)
+         _ _ _ _ _ πh₁ πh₁ (𝟙 _) _ _ _ _ _ _ _ _ _ _ _,
+        { simp only [eq_iff_true_of_subsingleton] },
+        { simp only [kernel.lift_ι] },
+        { simp only [pullback.lift_fst, category.comp_id] },
+        { simp only [category.id_comp, category.comp_id] },
+        { exact exact_zero_mono ιh₁ },
+        { exact (exact_iff_exact_seq _ _).2 (H₁.extract 0 2) },
+        { exact (exact_iff_exact_seq _ _).2 (H₁.extract 1 2) },
+        { exact exact_zero_mono (kernel.ι pullback.fst) },
+        { exact exact_kernel_ι },
+        { have : (pullback.fst : pullback g₂ f₂ ⟶ A₁₂) ≫ πh₁ = 0,
+          { apply zero_of_comp_mono gQh,
+            rw [category.assoc, sqᵣ.w, pullback.condition_assoc, (H₂.extract 1 2).w, comp_zero] },
+          apply abelian.exact_of_is_cokernel _ _ this,
+          have hex := (exact_iff_exact_seq _ _).2 (H₁.extract 1 2),
+          rw ← pullback.lift_fst _ _ sqm.w at hex,
+          exact is_colimit_of_is_colimit_comp (abelian.is_colimit_of_exact_of_epi _ _ hex) _ } } },
+    { apply is_colimit.of_point_iso (colimit.is_colimit _),
+      { apply_instance },
+      { let r := pushout.desc _ _ sqm.w,
+        let x : cokernel (pushout.inr : A₂₁ ⟶ pushout f₁ g₁) ⟶ Qh₂,
+        { refine cokernel.desc _ (r ≫ πh₂) _,
+          simp only [(H₂.extract 1 2).w, ← category.assoc, pushout.inr_desc] },
+        haveI : is_iso x,
+        { let psq := commsq.of_eq (@pushout.condition _ _ _ _ _ f₁ g₁ _),
+          let hcoker := abelian.is_colimit_of_exact_of_epi _ _
+            ((exact_iff_exact_seq _ _).2 (H₁.extract 1 2)),
+          obtain ⟨u : Qh₁ ⟶ _, hu⟩ := cokernel_cofork.is_colimit.desc' hcoker
+            (pushout.inl ≫ (cokernel.π (pushout.inr : A₂₁ ⟶ pushout f₁ g₁))) _,
+          { rw cofork.π_of_π at hu,
+            let lsq := commsq.of_eq hu,
+            haveI : is_iso u := is_iso_of_is_colimit u psq lsq _ _ _,
+            { have hxu : u ≫ x = gQh,
+              { simp only [← cancel_epi πh₁, hu, x, cokernel.π_desc, reassoc_of hu, r,
+                  pushout.inl_desc_assoc, sqᵣ.w] },
+              have hx : x = inv u ≫ gQh,
+              { rw [← is_iso.inv_comp_eq, is_iso.inv_inv, hxu] },
+              rw hx,
+              apply_instance },
+            { exact ((exact_iff_exact_seq _ _).2 (H₁.extract 1 2)) },
+            { exact exact_cokernel pushout.inr },
+            { exact pushout_is_pushout _ _ } },
+          { rw [← category.assoc, pushout.condition, category.assoc, cokernel.condition,
+              comp_zero] } },
+        refine @abelian.is_iso_of_is_iso_of_is_iso_of_is_iso_of_is_iso _ _ _ _ _ _ _ _ _ _ _
+          ιh₂ (pushout.inr : A₂₁ ⟶ pushout f₁ g₁) (cokernel.π (pushout.inr : A₂₁ ⟶ pushout f₁ g₁))
+          ιh₂ f₂ πh₂ (𝟙 _) (𝟙 _) r x _ _ _ 0 0 0 0 0 _ _ _ _ _ _ _ _ _ _ _,
+        { simp only [category.id_comp, category.comp_id] },
+        { simp only [category.id_comp, pushout.inr_desc] },
+        { simp only [cokernel.π_desc] },
+        { simp only [eq_iff_true_of_subsingleton] },
+        { have : ιh₂ ≫ (pushout.inr : A₂₁ ⟶ pushout f₁ g₁) = 0,
+          { apply zero_of_epi_comp gKh,
+            rw [← sqₗ.w_assoc, ← pushout.condition, reassoc_of (H₁.extract 0 2).w, zero_comp] },
+          apply abelian.exact_of_is_kernel _ _ this,
+          have hex := (exact_iff_exact_seq _ _).2 (H₂.extract 0 2),
+          rw ← pushout.inr_desc _ _ sqm.w at hex,
+          exact is_limit_of_is_limit_comp (abelian.is_limit_of_exact_of_mono _ _ hex) _ },
+        { exact exact_cokernel pushout.inr },
+        { exact exact_epi_zero (cokernel.π pushout.inr) },
+        { exact ((exact_iff_exact_seq _ _).2 (H₂.extract 0 2)) },
+        { exact ((exact_iff_exact_seq _ _).2 (H₂.extract 1 2)) },
+        { exact exact_epi_zero πh₂ } } } }
 end
